\documentclass[12pt]{article}
\usepackage[top=1in,left=1in,bottom=1in,right=1in,headsep=2pt]{geometry}	
\usepackage{amssymb,amsmath,amsthm,amsfonts}
\usepackage{chapterfolder,docmute,setspace}
\usepackage{cancel,multicol,tikz,verbatim,framed,polynom,enumitem}
\usepackage[colorlinks, hyperindex, plainpages=false, linkcolor=blue, urlcolor=blue, pdfpagelabels]{hyperref}
\usepackage[type={CC},modifier={by-sa},version={4.0},]{doclicense}

\theoremstyle{definition}
\newtheorem{example}{Example}
\newcommand{\Desmos}{\href{https://www.desmos.com/}{Desmos}}
\setlength{\parindent}{0em}
\setlist{itemsep=0em}
\setlength{\parskip}{0.1em}
\input{order}

\begin{document}
{\bf \large Lesson \arabic{lesson_elimination}: Solving Systems of Equations by Addition/Elimination}\phantomsection\label{les:elimination}\\
CC attribute: \href{http://www.wallace.ccfaculty.org/book/book.html}{\it{Beginning and Intermediate Algebra}} by T. Wallace. \hfill \doclicenseImage[imagewidth=5em]\\
\par
{\bf Objective:} Solve linear systems by addition and elimination.\\
\par
{\bf Students will be able to:}
\begin{itemize}
	\item Solve linear systems by addition and elimination of one variable.
	\item Write system solutions as ordered pairs in the form $(x,y)$.
	\item Verify the accuracy of a solution by plugging it into each equation in the system.
\end{itemize}
{\bf Prerequisite Knowledge:}
\begin{itemize}
	\item Solving a linear equation.
	\item Applying the distributive property.
	\item Combining like terms.
\end{itemize}
\hrulefill

{\bf Lesson:}
\par
{\bf I - Motivating Example(s):}\\
\ \par
We present the steps for solving a system of linear equations by addition/elimination alongside an example.
\begin{center}
\begin{tabular}{|l|l|}
  \hline
	& \\
  \ \ \ \ Steps for Addition/Elmination & \begin{tabular}{l}
    System: $\begin{cases}
		2 x - 5 y = -13\\
    -3y+4 = - 5x\end{cases}$
	\end{tabular}\\
  & \\
  \hline
  1. Line up the variables and constants. & \begin{tabular}{l}
    Rearrange the second equation\\
    $2 x - 5 y = - 13$\\
    $5 x - 3 y = - 4$\\
	\end{tabular}\\
  \hline
  2. Multiply to get opposites (use LCM). & $\begin{array}{l}
 
    \text{First Equation: multiply by} \ - 5\\
    - 5\cdot(2 x - 5 y) = (- 13)\cdot(- 5)\\
    ~- 10 x + 25 y = 65\\
 \\
   \text{Second Equation: multiply by} \ 2\\
    2\cdot (5 x - 3 y) = (- 4)\cdot 2\\
    ~~10 x - 6 y = - 8\\
  \end{array}$\\
  \hline
  3. Add equations to eliminate a variable.&  
	
	  $\begin{array}{l}
 ~~~~~- 10 x + 25 y = 65~~~~~~\\
 ~~~~~~\underline{~10 x~ -~ 6 y = - 8~~}\\
~~~~~~~~~~~~~~~~19 y =57\\
\end{array}$\\
\hline
\end{tabular}
\begin{tabular}{|l|l|}
  \hline
	4. Solve for the remaining variable. & $\begin{array}{l}
     ~~~~~~~~~~~~~~19y = 57\\
    ~~~~~~~~~~~~~~~\overline{19} ~~~~ \overline{19}\\
    ~~~~~~~~~~~~~~~~~y = 3
  \end{array}$\\
  \hline
  5.~$\begin{array}{l}
	\text{Plug back into either of the given equations}\\
	\text{and solve.}
	\end{array}$
	
& \begin{tabular}{l}
    ~~~~~~$2 x - 5 (3) = - 13$\\
    ~~~~~~~~$2 x - 15 = - 13$\\
    ~~~~~~~~~~~~~$\underline{+ 15 ~+ 15}$\\
		~~~~~~~~~~~~~~~$2 x = 2$\\
    ~~~~~~~~~~~~~~~~$\overline{2}$ ~~ $\overline{2}$\\
    ~~~~~~~~~~~~~~~~$x = 1$
  \end{tabular}\\
  \hline
  \ \ \ Our solution, as a coordinate pair. & ~~~~~~~~~~~~$(x,y)=(1, 3)$ \ \ \ \ \ \ \ \\
  \hline
\end{tabular}
\end{center}

{\bf II - Demo/Discussion Problems:}\\
\ \par
Solve each of the following systems of linear equations by addition/elimination.
\begin{multicols}{3}
	\begin{enumerate}
		\item $\begin{cases}
					3x+6y=-9\\
			    2x+9y=-26
					\end{cases}$
		\item $\begin{cases}
					2x-5y=3\\
					-6x+15y=-9
					\end{cases}$
		\item $\begin{cases}
					4 x - 6 y = 8\\
					6 x - 9 y = 15
					\end{cases}$
	\end{enumerate}
\end{multicols}
\ \par
{\bf III - Practice Problems:}\\
\ \par
Solve each of the following systems of linear equations by addition/elimination.
\begin{multicols}{3}
	\begin{enumerate}
  \item $\begin{cases}
	4 x + 2 y = 0\\
  - 4 x - 9 y = - 28
  \end{cases}$
  \item $\begin{cases}
	- 6 x + 9 y = 3\\
  6 x - 9 y = - 9
  \end{cases}$ 
  \item $\begin{cases}
  - x - 5 y = 28\\
  - x + 4 y = - 17
  \end{cases}$
  \item $\begin{cases}
  10 x + 6 y = 24\\
  - 6 x + y = 4
  \end{cases}$
  \item $\begin{cases}
  - 7 x + 4 y = - 4\\
  10 x - 8 y = - 8
  \end{cases}$
  \item $\begin{cases}
  - 7 x - 3 y = 12\\
  - 6 x - 5 y = 20
  \end{cases}$
  \item $\begin{cases}
  9 x + 6 y = - 21\\
  - 10 x - 9 y = 28
  \end{cases}$
  \item $\begin{cases}
  - 8 x - 8 y = - 8\\
  10 x + 9 y = 1
  \end{cases}$
  \item $\begin{cases}
  0 = 9 x + 5 y\\
  y = \frac{2}{7} x
	\end{cases}$
  \item $\begin{cases}
  - 7 x + y = - 10\\
  - 9 x - y = - 22
  \end{cases}$
  \item $\begin{cases}
  5 x - 5 y = - 15\\
  5 x - 5 y = - 15
  \end{cases}$
  \item $\begin{cases}
  - 10 x - 5 y = 0\\
  10 x +10 y=30
  \end{cases}$
  \item $\begin{cases}
  x + 3 y = - 1\\
  10 x + 6 y = - 10
  \end{cases}$
  \item $\begin{cases}
  - 6 x + 4 y = 4\\
  - 3 x - y = 26
  \end{cases}$
  \item $\begin{cases}
  - 5 x + 4 y = 4\\
  - 7 x - 10 y = - 10
  \end{cases}$
  \item $\begin{cases}
  - 4 x - 5 y = 12\\
  - 10 x + 6 y = 30
  \end{cases}$
  \item $\begin{cases}
  - 7 x + 10 y = 13\\
  4 x + 9 y = 22
  \end{cases}$
  \item $\begin{cases}
  - 6 - 42 y = - 12 x\\
	x - \frac{7}{2} y = \frac{1}{2} 
  \end{cases}$
  \item $\begin{cases}
  - 9 x + 5 y = - 22\\
  9 x - 5 y = 13
  \end{cases}$
  \item $\begin{cases}
  4 x - 6 y = - 10\\
  4 x - 6 y = - 14
  \end{cases}$
  \item $\begin{cases}
  2 x - y = 5\\
  5 x + 2 y = - 28
  \end{cases}$
  \item $\begin{cases}
  2 x + 4 y = 24\\
  4 x - 12 y = 8
  \end{cases}$
  \item $\begin{cases}
  5 x + 10 y = 20\\
  - 6 x - 5 y = - 3
  \end{cases}$
  \item $\begin{cases}
  9 x - 2 y = - 18\\
  5 x - 7 y = - 10
  \end{cases}$
  \item $\begin{cases}
  - 7 x + 5 y = - 8\\
  - 3 x - 3 y = 12
  \end{cases}$
  \item $\begin{cases}
  9 y = 7 - x\\
  - 18 y + 4 x = - 26
	\end{cases}$
  \item $\begin{cases}
  - x - 2 y = - 7\\
  x + 2 y = 7
  \end{cases}$
  \item $\begin{cases}
  - 3 x + 3 y = - 12\\
  - 3 x + 9 y = - 24
  \end{cases}$
  \item $\begin{cases}
  - 5 x + 6 y = - 17\\
  x - 2 y = 5
  \end{cases}$
  \item $\begin{cases}
  - 6 x + 4 y = 12\\
  12 x + 6 y = 18
  \end{cases}$
  \item $\begin{cases}
  - 9 x - 5 y = - 19\\
  3 x - 7 y = - 11
  \end{cases}$
  \item $\begin{cases}
  3 x + 7 y = - 8\\
  4 x + 6 y = - 4
  \end{cases}$
  \item $\begin{cases}
  8 x + 7 y = - 24\\
  6 x + 3 y = - 18
  \end{cases}$
  \item $\begin{cases}
  21 = - 9 x + 12 y\\
	\frac{4}{3} y + \frac{7}{3} x=-1
  \end{cases}$
	\end{enumerate}
\end{multicols}
\newpage
\ \newpage
\end{document}