\documentclass[12pt]{book}
\raggedbottom
\usepackage[top=1in,left=1in,bottom=1in,right=1in,headsep=0.25in]{geometry}	
\usepackage{amssymb,amsmath,amsthm,amsfonts}
\usepackage{chapterfolder,docmute,setspace}
\usepackage{cancel,multicol,tikz,verbatim,framed,polynom,enumitem,tikzpagenodes}
\usepackage[colorlinks, hyperindex, plainpages=false, linkcolor=blue, urlcolor=blue, pdfpagelabels]{hyperref}
\usepackage[type={CC},modifier={by-sa},version={4.0},]{doclicense}

\theoremstyle{definition}
\newtheorem{example}{Example}
\newcommand{\Desmos}{\href{https://www.desmos.com/}{Desmos}}
\setlength{\parindent}{0in}
\setlist{itemsep=0in}
\setlength{\parskip}{0.1in}
\setcounter{secnumdepth}{0}
\input{lesson_order}

\newcommand{\tmmathbf}[1]{\ensuremath{\boldsymbol{#1}}}
\newcommand{\tmop}[1]{\ensuremath{\operatorname{#1}}}

\begin{document}
\section{Practice Problems}
\subsection*{Graphing}
{\bf Solve each system by graphing.}

\begin{multicols}{3}
	\begin{enumerate}
	\item
	$\begin{cases}
	y = - x + 1\\
	y = - 5 x - 3
  \end{cases}$
	\item
	$\begin{cases}
	y = - \frac{3}{4} x + 1\\
	y = - \frac{3}{4} x + 2
  \end{cases}$
  \item
	$\begin{cases}
	y = \frac{5}{3} x + 4\\
	y = - \frac{2}{3} x - 3
  \end{cases}$
  \item
	$\begin{cases}
	x - y = 4\\
	2 x + y = - 1
  \end{cases}$
  \item
	$\begin{cases}
	2 x + y = 2\\
	x - y = 4
  \end{cases}$
  \item
	$\begin{cases}
	9y+6x=36\\
	3y-6x=-12
  \end{cases}$
  \item
	$\begin{cases}
	3 + y = - x\\
	- 4 - 6 x = - y
  \end{cases}$
	\item
	$\begin{cases}
	y = - \frac{5}{4} x - 2\\
	y = - \frac{1}{4} x + 2
  \end{cases}$
  \item
	$\begin{cases}
	y = 2 x + 2\\
	y = - x - 4
  \end{cases}$
  \item
	$\begin{cases}
	y = \frac{1}{2} x + 4\\
	y = \frac{1}{2} x + 1
  \end{cases}$
  \item
	$\begin{cases}
	6 x + y = - 3\\
	x + y = 2
  \end{cases}$
  \item
	$\begin{cases}
	x + 2 y = 6\\
	5 x - 4 y = 16
  \end{cases}$
  \item
	$\begin{cases}
	- 2 y + x = 4\\
	2 = - x + \frac{1}{2} y
  \end{cases}$
  \item
	$\begin{cases}
	16 = - x - 4 y\\
	- 2 x = - 4 - 4 y
  \end{cases}$
	\item
	$\begin{cases}
	y = - 3\\
	y = - x - 4
  \end{cases}$
  \item
	$\begin{cases}
	y = \frac{1}{3} x + 2\\
	y = - \frac{5}{3} x - 4
  \end{cases}$
  \item
	$\begin{cases}
	x + 3 y = - 9\\
	5 x + 3 y = 3
  \end{cases}$
  \item
	$\begin{cases}
	2 x + 3 y = - 6\\
	2 x + y = 2
  \end{cases}$
  \item
	$\begin{cases}
	2 x + y = - 2\\
	x + 3 y = 9
  \end{cases}$
  \item
	$\begin{cases}
	2 x - y = - 1\\
	3 = - 2 x - y
  \end{cases}$
  \item
	$\begin{cases}
	- y + 7 x = 4\\
	- y + 7 x = 3
  \end{cases}$
  \item
	$\begin{cases}
	y = - x - 2\\
	y = \frac{2}{3} x + 3
  \end{cases}$
  \item
	$\begin{cases}
	y = 2 x - 4\\
	y = \frac{1}{2} x + 2
  \end{cases}$
  \item
	$\begin{cases}
	x + 4 y = - 12\\
	2 x + y = 4
  \end{cases}$
  \item
	$\begin{cases}
	3 x + 2 y = 2\\
	3 x + 2 y = - 6
  \end{cases}$
  \item
	$\begin{cases}
	x - y = 3\\
	5 x + 2 y = 8
  \end{cases}$
	\item
	$\begin{cases}
	- 2 y = - 4 - x\\
	- 2 y = - 5 x + 4
  \end{cases}$
  \item
	$\begin{cases}
	- 4 + y = x\\
	x + 2 = - y
	\end{cases}$
	\end{enumerate}
\end{multicols}
\newpage
\subsection*{Substitution}
{\bf Solve each system by substitution.}
\begin{multicols}{3}
	\begin{enumerate}
  \item $\begin{cases} 
	y = - 3 x\\
	y = 6 x - 9
  \end{cases}$
  \item $\begin{cases} 
  y = 6 x + 4\\
	y = - 3 x - 5
  \end{cases}$
  \item $\begin{cases} 
  y = 2 x - 3\\
	y = - 2 x + 9
  \end{cases}$
  \item $\begin{cases} 
  y = - 6\\
	3 x - 6 y = 30
  \end{cases}$
  \item $\begin{cases} 
  - 2 x + 2 y = 18\\
  y = 7 x + 15
  \end{cases}$
  \item $\begin{cases} 
  7 x - 2 y = - 7\\
  y = 7
  \end{cases}$
  \item $\begin{cases} 
  - 2 x - y = - 5\\
  x - 8 y = - 23
  \end{cases}$
  \item $\begin{cases} 
  3 x + y = 9\\
	2 x + 8 y = - 16
  \end{cases}$
  \item $\begin{cases} 
  x + 5 y = 15\\
  - 3 x + 2 y = 6
  \end{cases}$
  \item $\begin{cases} 
  y = x + 5\\
	y = - 2 x - 4
  \end{cases}$
  \item $\begin{cases} 
  y = 3 x + 13\\
	y = - 2 x - 22
  \end{cases}$
  \item $\begin{cases} 
  y = 7 x - 24\\
	y = - 3 x + 16
  \end{cases}$
  \item $\begin{cases} 
  6 x - 4 y = - 8\\
  y = - 6 x + 2
  \end{cases}$
  \item $\begin{cases} 
  y = x + 4\\
	3 x - 4 y = - 19
  \end{cases}$
  \item $\begin{cases} 
  x - 2 y = - 13\\
  4 x + 2 y = 18
  \end{cases}$
  \item $\begin{cases} 
  6 x + 4 y = 16\\
  - 2 x + y = - 3
  \end{cases}$
  \item $\begin{cases} 
  - 5 x - 5 y = - 20\\
  - 2 x + y = 7
  \end{cases}$
  \item $\begin{cases} 
  2 x + 3 y = - 10\\
  7 x + y = 3
  \end{cases}$
  \item $\begin{cases} 
  y = - 2 x - 9\\
	y = 2 x - 1
  \end{cases}$
  \item $\begin{cases} 
  y = 3 x + 2\\
	y = - 3 x + 8
  \end{cases}$
  \item $\begin{cases} 
  y = 6 x - 6\\
	- 3 x - 3 y = - 24
  \end{cases}$
  \item $\begin{cases} 
  y = - 5\\
	3 x + 4 y = - 17
  \end{cases}$
  \item $\begin{cases} 
  y = - 8 x + 19\\
	- x + 6 y = 16
  \end{cases}$
  \item $\begin{cases} 
  x - 5 y = 7\\
	2 x + 7 y = - 20
  \end{cases}$
  \item $\begin{cases} 
  - 6 x + y = 20\\
  - 3 x - 3 y = - 18
  \end{cases}$
  \item $\begin{cases} 
  2 x + y = 2\\
  3 x + 7 y = 14
  \end{cases}$
  \item $\begin{cases} 
  - 2 x + 4 y = - 16\\
  y = - 2
  \end{cases}$
  \item $\begin{cases} 
  y = - 6 x + 3\\
	y = 6 x + 3
  \end{cases}$
  \item $\begin{cases} 
  y = - 2 x - 9\\
	y = - 5 x - 21
  \end{cases}$
  \item $\begin{cases} 
  - x + 3 y = 12\\
  y = 6 x + 21
  \end{cases}$
  \item $\begin{cases} 
  7 x + 2 y = - 7\\
  y = 5 x + 5
  \end{cases}$
  \item $\begin{cases} 
  y = - 2 x + 8\\
  - 7 x - 6 y = - 8
  \end{cases}$
  \item $\begin{cases} 
  3 x - 4 y = 15\\
  7 x + y = 4
  \end{cases}$
  \item $\begin{cases} 
  7 x + 5 y = - 13\\
  x - 4 y = - 16
  \end{cases}$
  \item $\begin{cases} 
  2 x + y = - 7\\
  5 x + 3 y = - 21
  \end{cases}$
  \item $\begin{cases} 
  - 2 x + 2 y = - 22\\
  - 5 x - 7 y = - 19
	\end{cases}$
	\end{enumerate}
\end{multicols}
\newpage
\subsection*{Addition Elimination}
{\bf Solve each system by elimination.}
\label{matrices1}
\begin{multicols}{3}
	\begin{enumerate}
  \item $\begin{cases}
	4 x + 2 y = 0\\
  - 4 x - 9 y = - 28
  \end{cases}$
  \item $\begin{cases}
	- 6 x + 9 y = 3\\
  6 x - 9 y = - 9
  \end{cases}$ 
  \item $\begin{cases}
  - x - 5 y = 28\\
  - x + 4 y = - 17
  \end{cases}$
  \item $\begin{cases}
  10 x + 6 y = 24\\
  - 6 x + y = 4
  \end{cases}$
  \item $\begin{cases}
  - 7 x + 4 y = - 4\\
  10 x - 8 y = - 8
  \end{cases}$
  \item $\begin{cases}
  - 7 x - 3 y = 12\\
  - 6 x - 5 y = 20
  \end{cases}$
  \item $\begin{cases}
  9 x + 6 y = - 21\\
  - 10 x - 9 y = 28
  \end{cases}$
  \item $\begin{cases}
  - 8 x - 8 y = - 8\\
  10 x + 9 y = 1
  \end{cases}$
  \item $\begin{cases}
  0 = 9 x + 5 y\\
  y = \frac{2}{7} x
	\end{cases}$
  \item $\begin{cases}
  - 7 x + y = - 10\\
  - 9 x - y = - 22
  \end{cases}$
  \item $\begin{cases}
  5 x - 5 y = - 15\\
  5 x - 5 y = - 15
  \end{cases}$
  \item $\begin{cases}
  - 10 x - 5 y = 0\\
  10 x +10 y=30
  \end{cases}$
  \item $\begin{cases}
  x + 3 y = - 1\\
  10 x + 6 y = - 10
  \end{cases}$
  \item $\begin{cases}
  - 6 x + 4 y = 4\\
  - 3 x - y = 26
  \end{cases}$
  \item $\begin{cases}
  - 5 x + 4 y = 4\\
  - 7 x - 10 y = - 10
  \end{cases}$
  \item $\begin{cases}
  - 4 x - 5 y = 12\\
  - 10 x + 6 y = 30
  \end{cases}$
  \item $\begin{cases}
  - 7 x + 10 y = 13\\
  4 x + 9 y = 22
  \end{cases}$
  \item $\begin{cases}
  - 6 - 42 y = - 12 x\\
	x - \frac{7}{2} y = \frac{1}{2} 
  \end{cases}$
  \item $\begin{cases}
  - 9 x + 5 y = - 22\\
  9 x - 5 y = 13
  \end{cases}$
  \item $\begin{cases}
  4 x - 6 y = - 10\\
  4 x - 6 y = - 14
  \end{cases}$
  \item $\begin{cases}
  2 x - y = 5\\
  5 x + 2 y = - 28
  \end{cases}$
  \item $\begin{cases}
  2 x + 4 y = 24\\
  4 x - 12 y = 8
  \end{cases}$
  \item $\begin{cases}
  5 x + 10 y = 20\\
  - 6 x - 5 y = - 3
  \end{cases}$
  \item $\begin{cases}
  9 x - 2 y = - 18\\
  5 x - 7 y = - 10
  \end{cases}$
  \item $\begin{cases}
  - 7 x + 5 y = - 8\\
  - 3 x - 3 y = 12
  \end{cases}$
  \item $\begin{cases}
  9 y = 7 - x\\
  - 18 y + 4 x = - 26
	\end{cases}$
  \item $\begin{cases}
  - x - 2 y = - 7\\
  x + 2 y = 7
  \end{cases}$
  \item $\begin{cases}
  - 3 x + 3 y = - 12\\
  - 3 x + 9 y = - 24
  \end{cases}$
  \item $\begin{cases}
  - 5 x + 6 y = - 17\\
  x - 2 y = 5
  \end{cases}$
  \item $\begin{cases}
  - 6 x + 4 y = 12\\
  12 x + 6 y = 18
  \end{cases}$
  \item $\begin{cases}
  - 9 x - 5 y = - 19\\
  3 x - 7 y = - 11
  \end{cases}$
  \item $\begin{cases}
  3 x + 7 y = - 8\\
  4 x + 6 y = - 4
  \end{cases}$
  \item $\begin{cases}
  8 x + 7 y = - 24\\
  6 x + 3 y = - 18
  \end{cases}$
  \item $\begin{cases}
  21 = - 9 x + 12 y\\
	\frac{4}{3} y + \frac{7}{3} x=-1
  \end{cases}$
	\end{enumerate}
\end{multicols}
\newpage
\subsection*{Three Variables}
{\bf Solve each of the following systems of equation.}
\label{matrices2}
\begin{multicols}{3}
\begin{enumerate}
	\item
	$\begin{cases}
2 x + y = z\\
4 x + z = 4 y\\
y = x + 1
  \end{cases}$
	\item
	$\begin{cases}
3 x + 2 y = z + 2\\
y = 1 - 2 x\\
3 z = - 2 y
  \end{cases}$
  	\item
	$\begin{cases}
x + y - z = 0\\
x - y - z = 0\\
x + y + 2 z = 0
  \end{cases}$
	\item
	$\begin{cases}
x + y - z = 0\\
x + 2 y - 4 z = 0\\
2 x + y + z = 0
  \end{cases}$
	\item
	$\begin{cases}
m + 6 n + 3 p = 8\\
3 m + 4 n = - 3\\
5 m + 7 n = 1
  \end{cases}$
	\item
	$\begin{cases}
2 x + 3 y = z - 1\\
3 x = 8 z - 1\\
5 y + 7 z = - 1
  \end{cases}$
	\item
	$\begin{cases}
x + 2 y - z = 4\\
4 x - 3 y + z = 8\\
5 x - y = 12
  \end{cases}$
	\item
	$\begin{cases}
4 x + 12 y + 16 z = 0\\
3 x + 4 y + 5 z = 0\\
x + 8 y + 11 z = 0
  \end{cases}$
	\item
	$\begin{cases}
2 x + y - 3 z = 0\\
x - 4 y + z = 0\\
4 x + 16 y + 4 z = 0
  \end{cases}$
  	\item
	$\begin{cases}
	a - 2 b + c = 5\\
    2 a + b - c = - 1\\
    3 a + 3 b - 2 c = - 4
    \end{cases}$
	\item
	$\begin{cases}
x + y + z = 2\\
6 x - 4 y + 5 z = 31\\
5 x + 2 y + 2 z = 13
    \end{cases}$
	\item
	$\begin{cases}
x + y + z = 6\\
2 x - y - z = - 3\\
x - 2 y + 3 z = 6
  \end{cases}$
	\item
	$\begin{cases}
p + q + r = 1\\
p + 2 q + 3 r = 4\\
4 p + 5 q + 6 r = 7
  \end{cases}$
	\item
	$\begin{cases}
x - y + 2 z = 0\\
x - 2 y + 3 z = - 1\\
2 x - 2 y + z = - 3
  \end{cases}$
	\item
	$\begin{cases}
x + 6 y + 3 z = 4\\
2 x + y + 2 z = 3\\
3 x - 2 y + z = 0
  \end{cases}$
	\item
	$\begin{cases}
- 2 x + y - 3 z = 1\\
x - 4 y + z = 6\\
4 x + 16 y + 4 z = 24
  \end{cases}$
	\item
	$\begin{cases}
x - 2 y + 3 z = 4\\
2 x - y + z = - 1\\
4 x + y + z = 1
  \end{cases}$
	\item
	$\begin{cases}
4 x - 7 y + 3 z = 1\\
3 x + y - 2 z = 4\\
4 x - 7 y + 3 z = 6
  \end{cases}$
	\item
	$\begin{cases}
3 x + y - z = 11\\
x + 3 y = z + 13\\
x + y - 3 z = 11
  \end{cases}$
	\item
	$\begin{cases}
x - y + 2 z = - 3\\
x + 2 y + 3 z = 4\\
2 x + y + z = - 3
  \end{cases}$
	\item
	$\begin{cases}
4 x + 12 y + 16 z = 4\\
3 x + 4 y + 5 z = 3\\
x + 8 y + 11 z = 1
  \end{cases}$
	\item
	$\begin{cases}
3 x + 2 y + 2 z = 3\\
x + 2 y - z = 5\\
2 x - 4 y + z = 0
  \end{cases}$
	\item
	$\begin{cases}
x + 2 y - 3 z = 9\\
2 x - y + 2 z = - 8\\
3 x - y - 4 z = 3
  \end{cases}$
	\item
	$\begin{cases}
4 x - 3 y + 2 z = 40\\
5 x + 9 y - 7 z = 47\\
9 x + 8 y - 3 z = 97
  	\end{cases}$
	\item
	$\begin{cases}
3 x + y - z = 10\\
8 x - y - 6 z = - 3\\
5 x - 2 y - 5 z = 1
  \end{cases}$
	\item
	$\begin{cases}
3 x + 3 y - 2 z = 13\\
6 x + 2 y - 5 z = 13\\
5 x - 2 y - 5 z = - 1
  \end{cases}$
	\item
	$\begin{cases}
2 x - 3 y + 5 z = 1\\
3 x + 2 y - z = 4\\
4 x + 7 y - 7 z = 7
	\end{cases}$
\phantomsection
\label{matrices3}
	\item
	$\begin{cases}
3 x - 4 y + 2 z = 1\\
2 x + 3 y - 3 z = - 1\\
x + 10 y - 8 z = 7
  \end{cases}$
	\item
	$\begin{cases}
2 w - 2 x - 2 y + 2 z = 10\\
w + x + y + z = - 5\\
3 w + 2 x + 2 y + 4 z = - 11\\
w + 3 x - 2 y + 2 z = - 6
	\end{cases}$
	\item
	$\begin{cases}
w - 2 x + 3 y - z = 8\\
w - x - y + z = 4\\
w + x + y + z = 22\\
w - x + y + z = 14
  \end{cases}$
	\item
	$\begin{cases}
w + x + y + z = 2\\
w + 2 x + 2 y + 4 z = 1\\
w - x + y + z = 6\\
w - 3 x - y + z = 2
  \end{cases}$
	\item
	$\begin{cases}
w + x - y + z = 0\\
- w + 2 x + 2 y + z = 5\\
w - 3 x - y + z = 4\\
2 w - x - y + 3 z = 7
	\end{cases}$
\end{enumerate}
\end{multicols}
\subsection*{Matrix Notation}
{\bf Construct an augmented matrix for each of the systems of equations referenced below.  Then row reduce your matrix to its row echelon form and determine if the given system has (1) no solution, (2) infinitely many solutions, or (3) exactly one solution.  If one solution exists, determine the reduced row echelon form for your matrix and use it to find the solution to the given system.}\par

1) - 5): Systems (1) through (5) on page \pageref{matrices1}.\par

6) - 10): Systems (11) through (15) on page \pageref{matrices1}.\par

11) - 20): Systems (1) through (10) on page \pageref{matrices2}.\par

21) - 24): Systems (29) through (32) on page \pageref{matrices3}.
\newpage
\end{document}