\documentclass[12pt]{article}
\usepackage[top=1in,left=1in,bottom=1in,right=1in,headsep=2pt]{geometry}	
\usepackage{amssymb,amsmath,amsthm,amsfonts}
\usepackage{chapterfolder,docmute,setspace}
\usepackage{cancel,multicol,tikz,verbatim,framed,polynom,enumitem}
\usepackage[colorlinks, hyperindex, plainpages=false, linkcolor=blue, urlcolor=blue, pdfpagelabels]{hyperref}
\usepackage[type={CC},modifier={by-sa},version={4.0},]{doclicense}

\theoremstyle{definition}
\newtheorem{example}{Example}
\newcommand{\Desmos}{\href{https://www.desmos.com/}{Desmos}}
\setlength{\parindent}{0em}
\setlist{itemsep=0em}
\setlength{\parskip}{0.1em}
\input{order}

\begin{document}
{\bf \large Lesson \arabic{lesson_substitution}: Solving Systems of Linear Equations by Substitution}\\
CC attribute: \href{http://www.wallace.ccfaculty.org/book/book.html}{\it{Beginning and Intermediate Algebra}} by T. Wallace. \hfill \doclicenseImage[imagewidth=5em]\\
\par
{\bf Objective:} Solve linear systems by substitution.\\
\par
{\bf Students will be able to:}
\begin{itemize}
	\item Identify a lone variable.
	\item Solve linear systems by substitution.
	\item Write system solutions as ordered pairs in the form $(x,y)$.
	\item Verify the accuracy of a solution by plugging it into each equation in the system.
\end{itemize}
{\bf Prerequisite Knowledge:}
\begin{itemize}
	\item Solving a linear equation.
	\item Applying the distributive property.
	\item Combining like terms.
\end{itemize}
\hrulefill

{\bf Lesson:}
\par
{\bf I - Motivating Example(s):}\\
\par
We present the steps for solving a system of linear equations by substitution alongside an example.
\begin{center}
\begin{tabular}{|l|c|}
  \hline
	& \\
  \ \ \ \ \ \ \ \ Steps for Substitution & \begin{tabular}{l}
    System: $\begin{cases}
		4 x - 2 y = 2\\
    2 x + y = - 5\end{cases}$
	\end{tabular}\\
  & \\
  \hline
  1. Identify a lone variable. & \begin{tabular}{l}
    The lone variable is $y$, in the\\
     second equation: $2 x + \framebox{$y$} = - 5$
  \end{tabular}\\
  \hline
  2. Solve for the lone variable. & \begin{tabular}{c}
    Subtract $2x$ from both sides.\\
    $y = - 5 - 2 x$
  \end{tabular}\\
  \hline
  3.~$\begin{array}{l}
	\text{Substitute into the untouched}\\
	\text{equation.}
	\end{array}$& $4 x - 2 (- 5 - 2 x)=2$\\
  \hline
  4. Solve for the remaining variable. & $\begin{array}{c}
 4 x + 10 + 4 x = 2~~~~~~~\\
 8 x + 10 = 2\\
 ~~~~~~~~\underline{- 10 ~~- 10}\\
~~~~~~~~~ 8 x = - 8\\
~~~~~~~~~ \overline{8} ~~~~~~ \overline{8}\\
~~~~~~~~~ x = - 1
  \end{array}$\\
  \hline
  5.~$\begin{array}{l}
	\text{Plug into lone variable}\\
	\text{equation and evaluate.}
	\end{array}$ & $\begin{array}{l}
    y = - 5 - 2 (- 1)\\
    y = - 5 + 2\\
    y = - 3
  \end{array}$\\
  \hline
  Our solution, as a coordinate pair. & $(x,y)=(- 1, - 3)$\\
  \hline
\end{tabular}
\end{center}

{\bf II - Demo/Discussion Problems:}\\
\ \par
Solve each of the following systems of linear equations by substitution.
\begin{multicols}{3}
	\begin{enumerate}
		\item $\begin{cases}
					2x-3y=7\\
			    y=3x-7
					\end{cases}$
		\item $\begin{cases}
					3x+2y=1\\
					x-5y=6
					\end{cases}$
		\item $\begin{cases}
			    x-y=2\\
				  8x-3y=16
					\end{cases}$
	\end{enumerate}
\end{multicols}
\ \par
{\bf III - Practice Problems:}\\
\ \par
Solve each of the following systems of linear equations by substitution.
\begin{multicols}{3}
	\begin{enumerate}
  \item $\begin{cases} 
	y = - 3 x\\
	y = 6 x - 9
  \end{cases}$
  \item $\begin{cases} 
  y = 6 x + 4\\
	y = - 3 x - 5
  \end{cases}$
  \item $\begin{cases} 
  y = 2 x - 3\\
	y = - 2 x + 9
  \end{cases}$
  \item $\begin{cases} 
  y = - 6\\
	3 x - 6 y = 30
  \end{cases}$
  \item $\begin{cases} 
  - 2 x + 2 y = 18\\
  y = 7 x + 15
  \end{cases}$
  \item $\begin{cases} 
  7 x - 2 y = - 7\\
  y = 7
  \end{cases}$
  \item $\begin{cases} 
  - 2 x - y = - 5\\
  x - 8 y = - 23
  \end{cases}$
  \item $\begin{cases} 
  3 x + y = 9\\
	2 x + 8 y = - 16
  \end{cases}$
  \item $\begin{cases} 
  x + 5 y = 15\\
  - 3 x + 2 y = 6
  \end{cases}$
  \item $\begin{cases} 
  y = x + 5\\
	y = - 2 x - 4
  \end{cases}$
  \item $\begin{cases} 
  y = 3 x + 13\\
	y = - 2 x - 22
  \end{cases}$
  \item $\begin{cases} 
  y = 7 x - 24\\
	y = - 3 x + 16
  \end{cases}$
  \item $\begin{cases} 
  6 x - 4 y = - 8\\
  y = - 6 x + 2
  \end{cases}$
  \item $\begin{cases} 
  y = x + 4\\
	3 x - 4 y = - 19
  \end{cases}$
  \item $\begin{cases} 
  x - 2 y = - 13\\
  4 x + 2 y = 18
  \end{cases}$
  \item $\begin{cases} 
  6 x + 4 y = 16\\
  - 2 x + y = - 3
  \end{cases}$
  \item $\begin{cases} 
  - 5 x - 5 y = - 20\\
  - 2 x + y = 7
  \end{cases}$
  \item $\begin{cases} 
  2 x + 3 y = - 10\\
  7 x + y = 3
  \end{cases}$
  \item $\begin{cases} 
  y = - 2 x - 9\\
	y = 2 x - 1
  \end{cases}$
  \item $\begin{cases} 
  y = 3 x + 2\\
	y = - 3 x + 8
  \end{cases}$
  \item $\begin{cases} 
  y = 6 x - 6\\
	- 3 x - 3 y = - 24
  \end{cases}$
  \item $\begin{cases} 
  y = - 5\\
	3 x + 4 y = - 17
  \end{cases}$
  \item $\begin{cases} 
  y = - 8 x + 19\\
	- x + 6 y = 16
  \end{cases}$
  \item $\begin{cases} 
  x - 5 y = 7\\
	2 x + 7 y = - 20
  \end{cases}$
  \item $\begin{cases} 
  - 6 x + y = 20\\
  - 3 x - 3 y = - 18
  \end{cases}$
  \item $\begin{cases} 
  2 x + y = 2\\
  3 x + 7 y = 14
  \end{cases}$
  \item $\begin{cases} 
  - 2 x + 4 y = - 16\\
  y = - 2
  \end{cases}$
  \item $\begin{cases} 
  y = - 6 x + 3\\
	y = 6 x + 3
  \end{cases}$
  \item $\begin{cases} 
  y = - 2 x - 9\\
	y = - 5 x - 21
  \end{cases}$
  \item $\begin{cases} 
  - x + 3 y = 12\\
  y = 6 x + 21
  \end{cases}$
  \item $\begin{cases} 
  7 x + 2 y = - 7\\
  y = 5 x + 5
  \end{cases}$
  \item $\begin{cases} 
  y = - 2 x + 8\\
  - 7 x - 6 y = - 8
  \end{cases}$
  \item $\begin{cases} 
  3 x - 4 y = 15\\
  7 x + y = 4
  \end{cases}$
  \item $\begin{cases} 
  7 x + 5 y = - 13\\
  x - 4 y = - 16
  \end{cases}$
  \item $\begin{cases} 
  2 x + y = - 7\\
  5 x + 3 y = - 21
  \end{cases}$
  \item $\begin{cases} 
  - 2 x + 2 y = - 22\\
  - 5 x - 7 y = - 19
	\end{cases}$
	\end{enumerate}
\end{multicols}
\newpage
\ \newpage
\end{document}